src/PulseTutorial.SpinLock.fst
@@ -1,60 +1,98 @@
-module PulseTutorial.SpinLock
+(*
+   Copyright 2023 Microsoft Research
 
+   Licensed under the Apache License, Version 2.0 (the "License");
+   you may not use this file except in compliance with the License.
+   You may obtain a copy of the License at
+
+       http://www.apache.org/licenses/LICENSE-2.0
+
+   Unless required by applicable law or agreed to in writing, software
+   distributed under the License is distributed on an "AS IS" BASIS,
+   WITHOUT WARRANTIES OR CONDITIONS OF ANY KIND, either express or implied.
+   See the License for the specific language governing permissions and
+   limitations under the License.
+*)
+
+module PulseTutorial.SpinLock
 #lang-pulse
-open Pulse
-module Box = Pulse.Lib.Box
+
+open Pulse.Lib.Pervasives
+
+module B = Pulse.Lib.Box
+
 module U32 = FStar.UInt32
 
-let maybe (b:bool) (p:vprop) =
+//lock$
+let maybe (b:bool) (p:slprop) =
   if b then p else emp
 
-let lock_inv (r:ref U32.t) (p:vprop) : v:vprop{is_big p ==> is_big v} =
-  exists* v. pts_to r v ** maybe (v = 0ul) p
+let lock_inv (r:B.box U32.t) (p:slprop) : slprop =
+  exists* v. B.pts_to r v ** maybe (v = 0ul) p
 
 noeq
-type lock (p:vprop) = {
-  r:ref U32.t;
-  i:iref;
+type lock = {
+  r:B.box U32.t;
+  i:iname;
 }
 
-let lock_alive #p (l:lock p) = inv l.i (lock_inv l.r p)
+let lock_alive (l:lock) (p:slprop) =
+  inv l.i (lock_inv l.r p)
+//end lock$
 
-fn new_lock (p:vprop)
-requires p ** pure (is_big p)
-returns  l:lock p
-ensures  lock_alive l
+ //dup_lock_alive$
+ghost
+fn dup_lock_alive (l:lock) (p:slprop)
+  requires lock_alive l p
+  ensures lock_alive l p ** lock_alive l p
 {
-   let r = Box.alloc 0ul;
-   Box.to_ref_pts_to r;
+  unfold lock_alive;
+  dup_inv l.i (lock_inv l.r p);
+  fold lock_alive;
+  fold lock_alive
+}
+//end dup_lock_alive$
+
+ //new_lock$
+fn new_lock (p:slprop)
+requires p
+returns l:lock
+ensures lock_alive l p
+{
+   let r = B.alloc 0ul;
    fold (maybe (0ul = 0ul) p);
-   fold (lock_inv (Box.box_to_ref r) p);
-   let i = new_invariant (lock_inv (Box.box_to_ref r) p);
-   let l = { r = Box.box_to_ref r; i } <: lock p;
-   rewrite each i as l.i;
-   fold (lock_alive l);
+   fold (lock_inv r p);
+   let i = new_invariant (lock_inv r p);
+   let l = {r;i};
+   rewrite (inv i (lock_inv r p)) as
+           (inv l.i (lock_inv l.r p));
+   fold lock_alive;
    l
 }
+//end new_lock$
 
-fn rec acquire #p (l:lock p)
-requires lock_alive l
-ensures  lock_alive l ** p
+
+//acquire_sig$
+fn rec acquire (#p:slprop) (l:lock)
+requires lock_alive l p
+ensures lock_alive l p ** p
+//end acquire_sig$
+//acquire_body$
 {
-  unfold (lock_alive l);
-  let b =
-    with_invariants l.i
-    returns b:bool
-    ensures maybe b p ** inv l.i (lock_inv l.r p)
-    {
+  unfold lock_alive;
+  let b = 
+    with_invariants bool emp_inames l.i (lock_inv l.r p)
+      emp (fun b -> maybe b p) fn _ {
       unfold lock_inv;
-      let b = cas l.r 0ul 1ul;
+      with vv. assert l.r |-> vv;
+      let b = cas_box l.r 0ul 1ul;
       if b
-      {
+      { 
         elim_cond_true _ _ _;
-        with _b. rewrite (maybe _b p) as p;
+        rewrite each vv as 0ul;
         fold (maybe false p);
         rewrite (maybe false p) as (maybe (1ul = 0ul) p);
         fold (lock_inv l.r p);
-        fold (maybe true p);
         true
       }
       else
@@ -65,25 +103,25 @@ ensures  lock_alive l ** p
         false
       }
     };
-  fold (lock_alive l);
+  fold lock_alive;
   if b { rewrite (maybe b p) as p; }
   else { rewrite (maybe b p) as emp; acquire l }
 }
+//end acquire_body$
 
-fn release #p (l:lock p)
-requires lock_alive l ** p
-ensures  lock_alive l
+//release$
+fn release (#p:slprop) (l:lock)
+requires lock_alive l p ** p
+ensures lock_alive l p
 {
-  unfold (lock_alive l);
-  with_invariants l.i
-    returns _:unit
-    ensures inv l.i (lock_inv l.r p)
-  {
+  unfold lock_alive;
+  with_invariants unit emp_inames l.i (lock_inv l.r p) p (fun _ -> emp) fn _ {
     unfold lock_inv;
-    write_atomic l.r 0ul;
-    drop_ (maybe _ _); // NB: Possible double release
+    write_atomic_box l.r 0ul;
+    drop_ (maybe _ _); //maybe release without acquire
     fold (maybe (0ul = 0ul) p);
     fold (lock_inv l.r p);
   };
-  fold (lock_alive l);
+  fold lock_alive
 }
+//end release$
