src/tutorial/PulseTutorial.Conditionals.fst
@@ -16,9 +16,9 @@
 
 module PulseTutorial.Conditionals
 #lang-pulse
-open Pulse
+open Pulse.Lib.Pervasives
 
-//SNIPPET_START: max$
+//max$
 let max_spec x y = if x < y then y else x
 
 fn max #p #q (x y:ref int)
@@ -38,9 +38,9 @@ ensures pts_to x #p 'vx ** pts_to y #q 'vy
         vy
     }
 }
-//SNIPPET_END: max$
+//end max$
 
-[@@expect_failure]
+//max_alt_fail$
 fn max_alt #p #q (x y:ref int)
 requires pts_to x #p 'vx ** pts_to y #q 'vy
 returns n:int
@@ -60,9 +60,11 @@ ensures pts_to x #p 'vx ** pts_to y #q 'vy
     };
     !result;
 }
+//end max_alt_fail$
 
 
-fn max_alt #p #q (x y:ref int)
+//max_alt$
+fn max_alt2 #p #q (x y:ref int)
 requires pts_to x #p 'vx ** pts_to y #q 'vy
 returns n:int
 ensures pts_to x #p 'vx ** pts_to y #q 'vy
@@ -87,23 +89,23 @@ ensures pts_to x #p 'vx ** pts_to y #q 'vy
     };
     !result;
 }
+//end max_alt$
 
 
-module T = FStar.Tactics
-
-//SNIPPET_START: nullable_ref$
-let nullable_ref a = option (ref a)
+//nullable_ref$
+let nullable_ref (a: Type0) = option (ref a)
 
 let pts_to_or_null #a
-        (x:nullable_ref a)
-        (#[default_arg (`full_perm)] p:perm) //implicit argument with a default
+        ([@@@mkey] x:nullable_ref a) 
+        (#[default_arg (`1.0R)] p:perm) //implicit argument with a default
         (v:option a)
-: vprop
+: slprop
 = match x with
   | None -> pure (v == None)
   | Some x -> exists* w. pts_to x #p w ** pure (v == Some w)
-//SNIPPET_END: nullable_ref$
+//end nullable_ref$
 
+//read_nullable$
 fn read_nullable #a #p (r:nullable_ref a)
 requires pts_to_or_null r #p 'v
 returns o:option a
@@ -112,7 +114,6 @@ ensures pts_to_or_null r #p 'v
 {
     match r {
      Some x -> {
-        rewrite each r as (Some x);
         unfold (pts_to_or_null (Some x) #p 'v);
         let o = !x;
         fold (pts_to_or_null (Some x) #p 'v);
@@ -120,16 +121,17 @@ ensures pts_to_or_null r #p 'v
         Some o
      }
      None -> {
-        rewrite each r as None;
         unfold (pts_to_or_null None #p 'v);
         fold (pts_to_or_null None #p 'v);
         rewrite each (None #(ref a)) as r;
-        None #a
+        None
      }
     }
 }
+//end read_nullable$
 
-//SNIPPET_START: pts_to_or_null_helpers$
+
+//pts_to_or_null_helpers$
 ghost
 fn elim_pts_to_or_null_none #a #p (r:nullable_ref a)
 requires pts_to_or_null r #p 'v ** pure (r == None)
@@ -164,11 +166,12 @@ fn intro_pts_to_or_null_some #a #p (r:nullable_ref a) (x:ref a)
 requires pts_to x #p 'v ** pure (r == Some x)
 ensures pts_to_or_null r #p (Some 'v)
 {
-    fold (pts_to_or_null (Some x) #p (Some 'v));
+    fold (pts_to_or_null (Some x) #p (Some (reveal 'v)));
     rewrite each (Some x) as r;
 }
-//SNIPPET_END: pts_to_or_null_helpers$
+//end pts_to_or_null_helpers$
 
+//read_nullable_alt$
 fn read_nullable_alt #a #p (r:nullable_ref a)
 requires pts_to_or_null r #p 'v
 returns o:option a
@@ -177,19 +180,22 @@ ensures pts_to_or_null r #p 'v
 {
     match r {
      Some x -> {
-        elim_pts_to_or_null_some r x;
+        elim_pts_to_or_null_some (Some x) x;
         let o = !x;
         intro_pts_to_or_null_some r x;
         Some o
      }
      None -> {
-        elim_pts_to_or_null_none r;
-        None #a
+        unfold pts_to_or_null None 'v;
+        fold pts_to_or_null None 'v;
+        rewrite each None #(ref a) as r;
+        None
      }
     }
 }
+//end read_nullable_alt$
 
-//SNIPPET_START: read_nullable_alt_fail$
+//read_nullable_alt_fail$
 [@@expect_failure]
 fn read_nullable_alt #a #p (r:nullable_ref a)
 requires pts_to_or_null r #p 'v
@@ -198,27 +204,32 @@ ensures emp
 {
     match r {
      Some x -> { admit () }
-     _ -> {
+     _ -> { 
         // we only have `r == _` in scope
         // not the negation of the prior branch conditions
         // i.e., unlike F*, we don't have not (Some? r)
         // so the assertion below fails
-        assert (pure (r == None));
+        assert (pure (r == None)); 
         admit() }
     }
 }
-//SNIPPET_END: read_nullable_alt_fail$
+//end read_nullable_alt_fail$
 
+//write_nullable$
 fn write_nullable #a (r:nullable_ref a) (v:a)
 requires pts_to_or_null r 'v
 ensures exists* w. pts_to_or_null r w ** pure (Some? r ==> w == Some v)
 {
     match r {
-     None -> { () }
+     None -> {
+        rewrite pts_to_or_null None 'v
+             as pts_to_or_null r 'v;
+     }
      Some x -> {
-        elim_pts_to_or_null_some r x;
+        unfold pts_to_or_null (Some x) 'v;
         x := v;
         intro_pts_to_or_null_some r x;
      }
     }
 }
+//end write_nullable$
