src/tutorial/PulseTutorial.Ghost.fst
@@ -16,7 +16,7 @@
 
 module PulseTutorial.Ghost
 #lang-pulse
-open Pulse
+open Pulse.Lib.Pervasives
 
 
 //incr_erased_non_ghost$
@@ -29,8 +29,9 @@ ensures emp ** pure (y == x + 1)
   let x = reveal x;
   (x + 1)
 }
-//incr_erased_non_ghost$
+//end incr_erased_non_ghost$
 
+//incr_erased$
 ghost
 fn incr_erased (x:erased int)
 requires emp
@@ -40,6 +41,8 @@ ensures emp ** pure (y == x + 1)
   let x = reveal x;
   (x + 1)
 }
+//end incr_erased$
+
 
 //try_use_incr_erased$
 [@@expect_failure]
@@ -50,7 +53,8 @@ ensures emp ** pure (y == x + 1)
 {
   incr_erased x;
 }
-//try_use_incr_erased$
+//end try_use_incr_erased$
+
 
 //use_incr_erased$
 fn use_incr_erased (x:erased int)
@@ -69,7 +73,9 @@ ensures emp ** pure (y == x + 1)
   };
   wrap x
 }
-//use_incr_erased$
+//end use_incr_erased$
+
+
 
 
 //use_incr_erased_alt$
@@ -77,10 +83,12 @@ fn use_incr_erased_alt (x:erased int)
 requires emp
 returns y:erased int
 ensures emp ** pure (y == x + 1)
-{
+{ 
   call_ghost incr_erased x;
 }
+//end use_incr_erased_alt$
 
+//add_erased$
 ghost
 fn add_erased (x y:erased int)
 requires emp
@@ -91,7 +99,10 @@ ensures emp ** pure (z == x + y)
   let y = reveal y;
   (x + y)
 }
+//end add_erased$
 
+
+//use_add_erased$
 fn use_add_erased (x y:erased int)
 requires emp
 returns z:erased int
@@ -99,7 +110,10 @@ ensures emp ** pure (z == x + y)
 {
   call_ghost (add_erased x) y
 }
+//end use_add_erased$
 
+
+//add_erased_erased$
 ghost
 fn add_erased_erased (x y:erased int)
 requires emp
@@ -110,79 +124,43 @@ ensures emp ** pure (z == x + y)
   let y = reveal y;
   hide (x + y)
 }
+//end add_erased_erased$
 
 let id p = p
 
 //__rewrite_sig$
 ghost
-fn __rewrite (p q:vprop)
+fn __rewrite (p q:slprop)
 requires p ** pure (p == q)
 ensures q
-//__rewrite_sig$
+//end __rewrite_sig$
 {
   rewrite p as q;
 }
 
+
+
 //intro_exists_sig$
 ghost
-fn intro_exists (#a:Type0) (p:a -> vprop) (x:erased a)
+fn intro_exists (#a:Type0) (p:a -> slprop) (x:erased a)
 requires p x
 ensures exists* x. p x
-//intro_exists_sig$
+//end intro_exists_sig$
 {
   ()
 }
 
+
 //all_at_most$
 let rec all_at_most (l:list (ref nat)) (n:nat)
-: vprop
+: slprop
 = match l with
   | [] -> emp
   | hd::tl -> exists* (i:nat). pts_to hd i ** pure (i <= n) ** all_at_most tl n
-//all_at_most$
-
-ghost
-fn elim_all_at_most_nil (l:list (ref nat)) (n:nat)
-requires all_at_most l n ** pure (l == [])
-ensures emp
-{
-  rewrite (all_at_most l n) as (all_at_most [] n);
-  unfold (all_at_most [] n);
-}
-
-ghost
-fn intro_all_at_most_nil (l:list (ref nat)) (n:nat)
-requires pure (l == [])
-ensures all_at_most l n
-{
-  fold (all_at_most [] n);
-  rewrite each (Nil #(ref nat)) as l;
-}
+//end all_at_most$
 
 
-ghost
-fn elim_all_at_most_cons (l:list (ref nat)) (hd:ref nat) (tl:list (ref nat)) (n:nat)
-requires all_at_most l n ** pure (l == hd :: tl)
-ensures exists* (i:nat). pts_to hd i ** pure (i <= n) ** all_at_most tl n
-{
-  rewrite (all_at_most l n) as (all_at_most (hd :: tl) n);
-  rewrite_by (all_at_most (hd::tl) n)
-             (exists* (i:nat). pts_to hd i ** pure (i <= n) ** all_at_most tl n)
-             vprop_equiv_norm ();
-}
-
-ghost
-fn intro_all_at_most_cons (l:list (ref nat)) (hd:ref nat) (tl:list (ref nat)) (n:nat)
-requires pts_to hd 'i ** all_at_most tl n ** pure ('i <= n) ** pure (l == hd :: tl)
-ensures all_at_most l n
-{
-  rewrite_by (exists* (i:nat). pts_to hd i ** pure (i <= n) ** all_at_most tl n)
-             (all_at_most (hd::tl) n)
-             vprop_equiv_norm ();
-  rewrite each (hd::tl) as l;
-}
-
-
+//weaken_at_most$
 ghost
 fn rec weaken_at_most (l:list (ref nat)) (n:nat) (m:nat)
 requires all_at_most l n ** pure (n <= m)
@@ -190,28 +168,35 @@ ensures all_at_most l m
 decreases l
 {
   match l {
-    Nil -> {
-      elim_all_at_most_nil l n;
-      intro_all_at_most_nil l m
+    [] -> {
+      unfold (all_at_most [] n);
+      fold (all_at_most [] m);
+      rewrite all_at_most [] m as all_at_most l m;
     }
-    Cons hd tl -> {
-      elim_all_at_most_cons l hd tl n;
+    hd :: tl -> {
+      unfold (all_at_most (hd::tl) n);
       weaken_at_most tl n m;
-      intro_all_at_most_cons l hd tl m
+      fold (all_at_most (hd::tl) m);
+      rewrite all_at_most (hd::tl) m as all_at_most l m;
     }
   }
 }
+//end weaken_at_most$
 
 module GR = Pulse.Lib.GhostReference
+//new_ghost_ref$
 ghost
-fn new_ghost_ref #a (x:a)
+fn new_ghost_ref (#a: Type0) (x:a)
 requires emp
 returns r:GR.ref a
 ensures GR.pts_to r x
 {
   GR.alloc x;
 }
+//end new_ghost_ref$
 
+
+//use_new_ghost_ref$
 fn use_new_ghost_ref (x:ref nat)
 requires pts_to x 'v
 returns r:GR.ref nat
@@ -220,28 +205,33 @@ ensures pts_to x 'v ** GR.pts_to r 'v
   let v = !x;
   new_ghost_ref v
 }
+//end use_new_ghost_ref$
+
 
 //correlated$
 let correlated #a (x:ref a) (y:GR.ref a) (v:a)=
-  pts_to x v ** GR.pts_to y #one_half v
-//correlated$
+  pts_to x v ** GR.pts_to y #0.5R v
+//end correlated$
+
 
 //use_temp_sig$
 fn use_temp (x:ref int) (y:GR.ref int)
 requires exists* v0. correlated x y v0
 ensures exists* v1. correlated x y v1
-//use_temp_sig$
+//end use_temp_sig$
 //use_temp_body$
 {
-  unfold correlated;
+  unfold correlated u#0;
   let v = !x;
   x := 17; //temporarily mutate x, give to to another function to use with full perm
   x := v; //but, we're forced to set it back to its original value
-  fold correlated;
+  fold correlated u#0;
 }
-//use_temp_body$
+//end use_temp_body$
 
 
+
+//use_correlated$
 fn use_correlated ()
 requires emp
 ensures emp
@@ -249,11 +239,12 @@ ensures emp
   let mut x = 17;
   let g = GR.alloc 17;
   GR.share g;
-  fold correlated;  // GR.pts_to g #one_half 17 ** correlated x g 17
-  use_temp x g;     // GR.pts_to g #one_half 17 ** correlated x g ?v1
-  unfold correlated; // GR.pts_to g #one_half 17 ** GR.pts_to g #one_half ?v1 ** pts_to x ?v1
+  fold correlated u#0;  // GR.pts_to g #0.5R 17 ** correlated x g 17
+  use_temp x g;     // GR.pts_to g #0.5R 17 ** correlated x g ?v1
+  unfold correlated u#0; // GR.pts_to g #0.5R 17 ** GR.pts_to g #0.5R ?v1 ** pts_to x ?v1
   GR.gather g;       //this is the crucial step
                      // GT.pts_to g 17 ** pure (?v1 == 17) ** pts_to x ?v1
   assert (pts_to x 17);
   GR.free g;
 }
+//end use_correlated$
