src/tutorial/PulseTutorial.LinkedList.fst
@@ -1,7 +1,23 @@
+(*
+   Copyright 2024 Microsoft Research
+
+   Licensed under the Apache License, Version 2.0 (the "License");
+   you may not use this file except in compliance with the License.
+   You may obtain a copy of the License at
+
+       http://www.apache.org/licenses/LICENSE-2.0
+
+   Unless required by applicable law or agreed to in writing, software
+   distributed under the License is distributed on an "AS IS" BASIS,
+   WITHOUT WARRANTIES OR CONDITIONS OF ANY KIND, either express or implied.
+   See the License for the specific language governing permissions and
+   limitations under the License.
+*)
+
+
 module PulseTutorial.LinkedList
 #lang-pulse
-open Pulse
-module S = Pulse.Lib.Stick.Util
+open Pulse.Lib.Pervasives
 module FA = Pulse.Lib.Forall.Util
 open FStar.List.Tot
 
@@ -16,29 +32,32 @@ and node_ptr (t:Type0) = ref (node t)
 
 //A nullable pointer to a node
 and llist (t:Type0) = option (node_ptr t)
-//llist$
+//end llist$
 
 //is_list$
-let rec is_list #t (x:llist t) (l:list t)
-: Tot vprop (decreases l)
+let rec is_list #t ([@@@mkey] x:llist t) (l:list t)
+: Tot slprop (decreases l)
 = match l with
   | [] -> pure (x == None)
-  | head::tl ->
+  | head::tl -> 
     exists* (p:node_ptr t) (tail:llist t).
       pure (x == Some p) **
       pts_to p { head; tail } **
       is_list tail tl
-//is_list$
+//end is_list$
 
 //boilerplate$
+
 ghost
 fn elim_is_list_nil (#t:Type0) (x:llist t)
-requires is_list x l ** pure (l == [])
+requires is_list x 'l ** pure ('l == [])
 ensures pure (x == None)
 {
-   rewrite each l as Nil #t;
+   rewrite each 'l as Nil #t;
    unfold (is_list x [])
 }
+
+
 
 ghost
 fn intro_is_list_nil (#t:Type0) (x:llist t)
@@ -47,6 +66,8 @@ ensures is_list x []
 {
     fold (is_list x []);
 }
+
+
 
 ghost
 fn elim_is_list_cons (#t:Type0) (x:llist t) (l:list t) (head:t) (tl:list t)
@@ -59,15 +80,10 @@ ensures (
 )
 {
   rewrite each l as (head::tl);
-  rewrite_by
-    (is_list x (head::tl))
-    (exists* (p:node_ptr t) (tail:llist t).
-      pure (x == Some p) **
-      pts_to p { head; tail } **
-      is_list tail tl)
-    vprop_equiv_norm
-    ()
+  unfold (is_list x (head::tl));
 }
+
+    
 
 
 ghost
@@ -80,42 +96,37 @@ ensures
   is_list x (node.head::tl)
 {
     rewrite (pts_to v node) as (pts_to v { head=node.head; tail=node.tail });
-    rewrite_by
-        (exists* (v:node_ptr t) (tail:llist t).
-          pure (x == Some v) **
-          pts_to v { head=node.head; tail } **
-          is_list tail tl)
-        (is_list x (node.head::tl))
-        vprop_equiv_norm
-        ()
+    fold (is_list x (node.head::tl));
 }
-//boilerplate$
+
+//end boilerplate$
 
 //is_list_cases$
 let is_list_cases #t (x:llist t) (l:list t)
-: vprop
+: slprop 
 = match x with
   | None -> pure (l == [])
-  | Some v ->
+  | Some v -> 
     exists* (n:node t) (tl:list t).
       pts_to v n **
       pure (l == n.head::tl) **
       is_list n.tail tl
-//is_list_cases$
+//end is_list_cases$
 
+//cases_of_is_list$
 ghost
 fn cases_of_is_list #t (x:llist t) (l:list t)
 requires is_list x l
 ensures is_list_cases x l
 {
   match l {
-    Nil -> {
-      elim_is_list_nil x;
+    [] -> {
+      unfold (is_list x []);
       fold (is_list_cases None l);
       rewrite each (None #(ref (node t))) as x;
     }
-    Cons head tl -> {
-      elim_is_list_cons x l head tl;
+    head :: tl -> {
+      unfold (is_list x (head::tl));
       with w tail. _;
       let v = Some?.v x;
       rewrite each w as v;
@@ -125,7 +136,10 @@ ensures is_list_cases x l
     }
   }
 }
+//end cases_of_is_list$
 
+
+//is_list_case_none$
 ghost
 fn is_list_case_none (#t:Type) (x:llist t) (#l:list t)
 requires is_list x l ** pure (x == None)
@@ -134,12 +148,15 @@ ensures is_list x l ** pure (l == [])
   cases_of_is_list x l;
   rewrite each x as (None #(ref (node t)));
   unfold (is_list_cases None l);
-  intro_is_list_nil x;
+  fold (is_list x []);
+  rewrite is_list x [] as is_list x l;
 }
+//end is_list_case_none$
 
 
+//is_list_case_some$
 ghost
-fn is_list_case_some (#t:Type) (x:llist t) (v:node_ptr t) (#l:list t)
+fn is_list_case_some (#t:Type) (x:llist t) (v:node_ptr t) (#l:list t) 
 requires is_list x l ** pure (x == Some v)
 ensures
   exists* (node:node t) (tl:list t).
@@ -151,75 +168,62 @@ ensures
   rewrite each x as (Some v);
   unfold (is_list_cases (Some v) l);
 }
+//end is_list_case_some$
 
 
+
+//length$
 fn rec length (#t:Type0) (x:llist t)
 requires is_list x 'l
 returns n:nat
 ensures is_list x 'l ** pure (n == List.Tot.length 'l)
 {
   match x {
-    None -> {
+    norewrite None -> {
       is_list_case_none x;
       0
     }
-    Some vl -> {
+    norewrite Some vl -> {
       is_list_case_some x vl;
-      with _node _tl. _;
       let node = !vl;
-      rewrite each _node as node;
       let n = length node.tail;
       intro_is_list_cons x vl;
       (1 + n)
     }
   }
 }
+//end length$
 
+
+
+//length_tail$
 fn rec length_tail (#t:Type0) (x:llist t) (k:nat)
 requires is_list x 'l
 returns n:nat
 ensures is_list x 'l ** pure (n == k + List.Tot.length 'l)
 {
   match x {
-    None -> {
+    norewrite None -> {
       is_list_case_none x;
       k
     }
-    Some vl -> {
+    norewrite Some vl -> {
       is_list_case_some x vl;
       with _node _tl. _;
       let n = !vl;
-      rewrite each _node as n;
       let n = length_tail n.tail (1 + k);
       intro_is_list_cons x vl;
       n
     }
   }
 }
+//end length_tail$
 
-module I = Pulse.Lib.Stick.Util
+
+module I = Pulse.Lib.Trade.Util
 open I
 
-ghost
-fn tail_for_cons (#t:Type) (v:node_ptr t) (#n:node t) (tl:erased (list t))
-requires
-  pts_to v n
-ensures
-  (is_list n.tail tl @==> is_list (Some v) (n.head::tl))
-{
-  ghost
-  fn aux ()
-  requires
-    pts_to v n ** is_list n.tail tl
-  ensures
-    is_list (Some v) (n.head::tl)
-  {
-    intro_is_list_cons (Some v) v
-  };
-  I.intro _ _ _ aux;
-}
-
-
+//tail$
 fn tail (#t:Type) (x:llist t)
 requires is_list x 'l ** pure (Some? x)
 returns y:llist t
@@ -227,16 +231,19 @@ ensures exists* tl.
     is_list y tl **
     (is_list y tl @==> is_list x 'l) **
     pure (Cons? 'l /\ tl == Cons?.tl 'l)
-{
+{ 
     let np = Some?.v x;
     is_list_case_some x np;
-    with node tl. _;
     let nd = !np;
-    rewrite each node as nd;
-    tail_for_cons np tl;
+    with tl. assert is_list nd.tail tl;
+    intro (is_list nd.tail tl @==> is_list x 'l) #(np |-> nd) fn _ {
+      intro_is_list_cons x np;
+    };
     nd.tail
 }
+//end tail$
 
+//length_iter$
 fn length_iter (#t:Type) (x: llist t)
 requires is_list x 'l
 returns n:nat
@@ -244,25 +251,21 @@ ensures is_list x 'l ** pure (n == List.Tot.length 'l)
 {
   open I;
   let mut cur = x;
-  let mut ctr = 0;
+  let mut ctr = 0; 
   I.refl (is_list x 'l); //initialize the trade for the invariant
   while (
-    let v = !cur;
-    Some? v
+    Some? !cur
   )
-  invariant b.
+  invariant
   exists* n ll suffix.
     pts_to ctr n **
     pts_to cur ll **
     is_list ll suffix **
-    pure (n == List.Tot.length 'l - List.Tot.length suffix /\
-          b == (Some? ll)) **
+    pure (n == List.Tot.length 'l - List.Tot.length suffix) **
     (is_list ll suffix @==> is_list x 'l)
   {
-    with _n _ll _suffix. _; //bind existential variables in the invariant
     let n = !ctr;
     let ll = !cur;
-    rewrite each _ll as ll; //again, rewrite the context to use ll instead of _ll
     let next = tail ll;     //tail gives us back a trade
     with tl. _;
     I.trans (is_list next tl) _ _; //extend the trade, transitively
@@ -275,23 +278,22 @@ ensures is_list x 'l ** pure (n == List.Tot.length 'l)
   let n = !ctr;
   n
 }
+//end length_iter$
 
+//append$
 fn rec append (#t:Type0) (x y:llist t)
 requires is_list x 'l1 ** is_list y 'l2 ** pure (Some? x)
 ensures is_list x ('l1 @ 'l2)
 {
   let np = Some?.v x;
   is_list_case_some x np;
-  with _node _tl. _;
   let node = !np;
-  rewrite each _node as node;
   match node.tail {
     None -> {
       is_list_case_none node.tail;
       elim_is_list_nil node.tail;
       np := { node with tail = y };
-      rewrite each y as ({ node with tail = y }).tail in (is_list y 'l2);
-      intro_is_list_cons x np;
+      intro_is_list_cons x np; 
     }
     Some _ -> {
       append node.tail y;
@@ -299,7 +301,11 @@ ensures is_list x ('l1 @ 'l2)
     }
   }
 }
+//end append$
 
+//tail_alt$
+let is_cons #t ([@@@mkey] x: list t) (hd: t) (tl: list t) : slprop =
+  pure (x == hd :: tl)
 
 fn tail_alt (#t:Type) (x:llist t)
 requires is_list x 'l ** pure (Some? x)
@@ -307,24 +313,22 @@ returns y:llist t
 ensures exists* hd tl.
   is_list y tl **
   (forall* tl'. is_list y tl' @==> is_list x (hd::tl')) **
-  pure ('l == hd::tl)
-{
+  is_cons 'l hd tl
+{ 
   let np = Some?.v x;
   is_list_case_some x np;
   with _node _tl. _;
   let node = !np;
-  rewrite each _node as node;
-  ghost
-  fn aux (tl':list t)
-    requires pts_to np node ** is_list node.tail tl'
-    ensures is_list x (node.head::tl')
-  {
+  intro (forall* tl'. is_list node.tail tl' @==> is_list x (node.head::tl'))
+      #(pts_to np node) fn _ tl' {
     intro_is_list_cons x np;
   };
-  FA.intro_forall_imp _ _ _ aux;
+  fold is_cons 'l node.head _tl;
   node.tail
 }
+//end tail_alt$
 
+//is_last_cell$
 fn is_last_cell (#t:Type) (x:llist t)
 requires is_list x 'l ** pure (Some? x)
 returns b:bool
@@ -332,16 +336,14 @@ ensures is_list x 'l ** pure (b == (List.Tot.length 'l = 1))
 {
   let np = Some?.v x;
   is_list_case_some x np;
-  with _node _tl. _;
   let node = !np;
-  rewrite each _node as node;
   match node.tail {
-    None -> {
+    None -> { 
       is_list_case_none node.tail;
       intro_is_list_cons x np;
       true
     }
-    Some vtl -> {
+    Some vtl -> { 
       is_list_case_some node.tail vtl;
       intro_is_list_cons node.tail vtl;
       intro_is_list_cons x np;
@@ -349,8 +351,9 @@ ensures is_list x 'l ** pure (b == (List.Tot.length 'l = 1))
     }
   }
 }
+//end is_last_cell$
 
-
+//append_at_last_cell$
 fn append_at_last_cell (#t:Type) (x y:llist t)
 requires
   is_list x 'l1 **
@@ -366,9 +369,11 @@ ensures
   let node = !np;
   np := { node with tail = y };
   rewrite each y as ({node with tail = y}).tail in (is_list y 'l2);
-  intro_is_list_cons x np;
+  intro_is_list_cons x np; 
 }
+//end append_at_last_cell$
 
+//non_empty_list$
 ghost
 fn non_empty_list (#t:Type0) (x:llist t)
 requires is_list x 'l ** pure (Cons? 'l)
@@ -380,63 +385,58 @@ ensures is_list x 'l ** pure (Some? x)
     rewrite each tail as n.tail;
     intro_is_list_cons x v #n #tl;
 }
+//end non_empty_list$
 
+fn not_is_last_cell (#t:Type) (x:llist t)
+requires is_list x 'l ** pure (Some? x)
+returns b:bool
+ensures is_list x 'l ** pure (b == (List.Tot.length 'l <> 1))
+{
+  not (is_last_cell x)
+}
 
+//append_iter$
 fn append_iter (#t:Type) (x y:llist t)
 requires is_list x 'l1 ** is_list y 'l2 ** pure (Some? x)
 ensures is_list x ('l1 @ 'l2)
 {
   let mut cur = x;
   //the base case, set up the initial invariant
-  FA.intro emp (fun l -> I.refl (is_list x l));
-  rewrite (forall* l. is_list x l @==> is_list x l)
-      as  (forall* l. is_list x l @==> is_list x ([]@l));
-  while (
-    with _b ll pfx sfx. _;
-    let l = !cur;
-    rewrite each ll as l;
-    let b = is_last_cell l; //check if we are at the last cell
-    if b
-    {
-      false //yes, break out of the loop
-    }
-    else
-    {
-      let next = tail_alt l;
-      with hd tl. _;
-      (* this is the key induction step *)
-      FA.trans_compose
-          (is_list next) (is_list l) (is_list x)
-          (fun tl -> hd :: tl)
-          (fun tl -> pfx @ tl);
-      //Use F* sugar for classical connectives to introduce a property
-      //needed for the next rewrite
-      (introduce forall tl. pfx @ (hd :: tl) == (pfx @ [hd]) @ tl
-       with List.Tot.Properties.append_assoc pfx [hd] tl);
-      rewrite (forall* tl. is_list next tl @==> is_list x (pfx@(hd::tl)))
-           as (forall* tl. is_list next tl @==> is_list x ((pfx@[hd])@tl));
-      cur := next;
-      non_empty_list next; //need to prove that Some? next, for the invariant
-      true
-    }
-  )
-  invariant b.
-  exists* ll pfx sfx.
+  intro (forall* l. is_list x l @==> is_list x ([] @ l)) fn _ l {};
+  while (not_is_last_cell (!cur)) //check if we are at the last cell
+  invariant exists* ll pfx sfx.
     pts_to cur ll **   //cur holds the pointer to the current head of the traversal, ll
     is_list ll sfx **  //ll points to some suffix of the original list, since `pfx@sfx = 'l1` below
-    //the main bit: whatever ll points to `sfx'`, trade it for x pointing to the concatenation ``pfx @ sfx'``
-    (forall* sfx'. is_list ll sfx' @==> is_list x (pfx @ sfx')) **
+    //the main bit: whatever ll points to `sfx'`, trade it for x pointing to the concatenation ``pfx @ sfx'`` 
+    (forall* sfx'. is_list ll sfx' @==> is_list x (pfx @ sfx')) ** 
     pure (
-      (b==false ==> List.Tot.length sfx == 1) /\ //the loop ends when we reach the last cell
       pfx@sfx == 'l1 /\ //sfx is really the suffix
       Some? ll          //and the current list is always non-null
     )
-  { () };
+  {
+    with ll pfx sfx. _;
+    let l = !cur;
+    let next = tail_alt l;
+    with hd tl. unfold is_cons sfx hd tl;
+    (* this is the key induction step *)
+    FA.trans_compose
+        (is_list next) (is_list l) (is_list x)
+        (fun tl -> hd :: tl)
+        (fun tl -> pfx @ tl);
+    //Use F* sugar for classical connectives to introduce a property
+    //needed for the next rewrite
+    (introduce forall tl. pfx @ (hd :: tl) == (pfx @ [hd]) @ tl
+      with List.Tot.Properties.append_assoc pfx [hd] tl);
+    rewrite (forall* tl. is_list next tl @==> is_list x (pfx@(hd::tl)))
+          as (forall* tl. is_list next tl @==> is_list x ((pfx@[hd])@tl));
+    cur := next;
+    non_empty_list next; //need to prove that Some? next, for the invariant
+  };
   with ll pfx sfx. _;
   let last = !cur;
-  rewrite each ll as last;
   append_at_last_cell last y;
   FA.elim_forall_imp (is_list last) (fun sfx' -> is_list x (pfx @ sfx')) (sfx@'l2);
   List.Tot.Properties.append_assoc pfx sfx 'l2;
   ()
 }
+//end append_iter$
