src/tutorial/PulseTutorial.ParallelIncrement.fst
@@ -1,24 +1,38 @@
+(*
+   Copyright 2023 Microsoft Research
+
+   Licensed under the Apache License, Version 2.0 (the "License");
+   you may not use this file except in compliance with the License.
+   You may obtain a copy of the License at
+
+       http://www.apache.org/licenses/LICENSE-2.0
+
+   Unless required by applicable law or agreed to in writing, software
+   distributed under the License is distributed on an "AS IS" BASIS,
+   WITHOUT WARRANTIES OR CONDITIONS OF ANY KIND, either express or implied.
+   See the License for the specific language governing permissions and
+   limitations under the License.
+*)
+
 module PulseTutorial.ParallelIncrement
 #lang-pulse
-open Pulse
-module U32 = FStar.UInt32
+open Pulse.Lib.Pervasives
+open Pulse.Lib.Par
 module L = Pulse.Lib.SpinLock
 module GR = Pulse.Lib.GhostReference
-module R = Pulse.Lib.Reference
 
+//par$
 fn par (#pf #pg #qf #qg:_)
+       {| is_send pf, is_send pg, is_send qf, is_send qg |}
        (f: unit -> stt unit pf (fun _ -> qf))
        (g: unit -> stt unit pg (fun _ -> qg))
 requires pf ** pg
 ensures qf ** qg
 {
-  parallel
-  requires pf and pg
-  ensures qf and qg
-  { f () }
-  { g () };
-  ()
+  par f g
 }
+//end par$
+
 
 fn incr2 (x y:ref int)
 requires pts_to x 'i ** pts_to y 'j
@@ -31,8 +45,9 @@ ensures pts_to x ('i + 1) ** pts_to y ('j + 1)
     let v = !x;
     x := v + 1;
   };
-  par (fun _ -> incr x) (fun _ -> incr y);
+  par (fun _ -> incr x #'i) (fun _ -> incr y #'j);
 }
+
 
 
 [@@expect_failure]
@@ -50,43 +65,52 @@ ensures pts_to x ('i + 2)
   par (fun _ -> incr) (fun _ -> incr);
 }
 
+
+//attempt$
 fn attempt (x:ref int)
 requires pts_to x 'i
-ensures emp
+ensures exists* v. pts_to x v
 {
-  let l = L.new_lock (exists* v. pts_to x v);
+  let l = L.new_lock (exists* (v: int). pts_to x v);
   fn incr ()
-  requires emp
-  ensures emp
+  requires L.lock_alive l #0.5R (exists* v. pts_to x v)
+  ensures L.lock_alive l #0.5R (exists* v. pts_to x v)
   {
     L.acquire l;
     let v = !x;
     x := v + 1;
     L.release l
   };
-  par incr incr
+  L.share l;
+  par incr incr;
+  L.gather l;
+  L.acquire l;
+  L.free l
 }
+//end attempt$
 
 //lock_inv$
-let contributions (left right: GR.ref int) (i v:int)=
+let contributions (left right: GR.ref int) (i v:int) : timeless_slprop =
   exists* (vl vr:int).
-    GR.pts_to left #one_half vl **
-    GR.pts_to right #one_half vr **
+    GR.pts_to left #0.5R vl **
+    GR.pts_to right #0.5R vr **
     pure (v == i + vl + vr)
 
-let lock_inv (x:ref int) (init:int) (left right:GR.ref int) =
-  exists* v.
+let lock_inv (x:ref int) (init:int) (left right:GR.ref int) : timeless_slprop =
+  exists* v. 
     pts_to x v **
     contributions left right init v
-//lock_inv$
+//end lock_inv$
 
+//incr_left$
 fn incr_left (x:ref int)
+             (#p:perm)
              (#left:GR.ref int)
              (#right:GR.ref int)
              (#i:erased int)
-             (lock:L.lock (lock_inv x i left right))
-requires GR.pts_to left #one_half 'vl
-ensures  GR.pts_to left #one_half ('vl + 1)
+             (lock:L.lock )
+requires L.lock_alive lock #p (lock_inv x i left right) ** GR.pts_to left #0.5R 'vl
+ensures L.lock_alive lock #p (lock_inv x i left right) ** GR.pts_to left #0.5R ('vl + 1)
 {
   L.acquire lock;
   unfold lock_inv;
@@ -97,17 +121,20 @@ ensures  GR.pts_to left #one_half ('vl + 1)
   GR.write left ('vl + 1);
   GR.share left;
   fold (contributions left right i (v + 1));
-  fold lock_inv;
+  fold lock_inv x i left right;
   L.release lock
 }
+//end incr_left$
 
+//incr_right$
 fn incr_right (x:ref int)
+              (#p:perm)
               (#left:GR.ref int)
               (#right:GR.ref int)
               (#i:erased int)
-              (lock:L.lock (lock_inv x i left right))
-requires GR.pts_to right #one_half 'vl
-ensures  GR.pts_to right #one_half ('vl + 1)
+              (lock:L.lock)
+requires L.lock_alive lock #p (lock_inv x i left right) ** GR.pts_to right #0.5R 'vl
+ensures L.lock_alive lock #p (lock_inv x i left right) ** GR.pts_to right #0.5R ('vl + 1)
 {
   L.acquire lock;
   unfold lock_inv;
@@ -121,7 +148,9 @@ ensures  GR.pts_to right #one_half ('vl + 1)
   fold (lock_inv x i left right);
   L.release lock
 }
+//end incr_right$
 
+//add2$
 fn add2 (x:ref int)
 requires pts_to x 'i
 ensures  pts_to x ('i + 2)
@@ -133,9 +162,12 @@ ensures  pts_to x ('i + 2)
   fold (contributions left right 'i 'i);
   fold (lock_inv x 'i left right);
   let lock = L.new_lock (lock_inv x 'i left right);
-  par (fun _ -> incr_left x lock)
-      (fun _ -> incr_right x lock);
+  L.share lock;
+  par (fun _ -> incr_left x #0.5R #left #right #'i lock #0)
+      (fun _ -> incr_right x #0.5R #left #right #'i lock #0);
+  L.gather lock;
   L.acquire lock;
+  L.free lock;
   unfold lock_inv;
   unfold contributions;
   GR.gather left;
@@ -143,6 +175,7 @@ ensures  pts_to x ('i + 2)
   GR.free left;
   GR.free right;
 }
+//end add2$
 
 /////////////////////////////////////////////////////////////////////////
 // A bit more generic, with ghost functions
@@ -151,27 +184,31 @@ ensures  pts_to x ('i + 2)
 
 //Parameterize incr by the ghost steps it needs to take
 //give it an abstract spec in terms of some call-provided aspec
+//incr$
+[@@erasable]
+let incr_f (x: ref int) (refine aspec: int -> slprop) =
+  v:int -> vq:int -> stt_ghost unit emp_inames
+    (refine v ** aspec vq ** pts_to x (v + 1))
+    (fun _ -> refine (v + 1) ** aspec (vq + 1) ** pts_to x (v + 1))
 fn incr (x: ref int)
-        (#refine #aspec: int -> vprop)
-        (l:L.lock (exists* v. pts_to x v ** refine v))
-        (ghost_steps:
-          (v:int -> vq:int -> stt_ghost unit emp_inames
-               (refine v ** aspec vq ** pts_to x (v + 1))
-               (fun _ -> refine (v + 1) ** aspec (vq + 1) ** pts_to x (v + 1))))
-requires aspec 'i
-ensures aspec ('i + 1)
+        (#p:perm)
+        (#refine #aspec: int -> slprop)
+        (l:L.lock)
+        (ghost_steps: incr_f x refine aspec)
+requires L.lock_alive l #p (exists* v. pts_to x v ** refine v) ** aspec 'i
+ensures L.lock_alive l #p (exists* v. pts_to x v ** refine v) ** aspec ('i + 1)
  {
     L.acquire l;
-    with _v. _;
     let vx = !x;
-    rewrite each _v as vx;
     x := vx + 1;
     ghost_steps vx 'i;
     L.release l;
 }
+//end incr$
 
 //At the call-site, we instantiate incr twice, with different
 //ghost steps
+//add2_v2$
 fn add2_v2 (x: ref int)
 requires pts_to x 'i
 ensures pts_to x ('i + 2)
@@ -189,23 +226,18 @@ ensures pts_to x ('i + 2)
     fn step
         (lr:GR.ref int)
         (b:bool { if b then lr == left else lr == right })
-        (v vq:int)
-      requires
-        contributions left right 'i v **
-        GR.pts_to lr #one_half vq **
-        pts_to x (v + 1)
-      ensures
-        contributions left right 'i (v + 1) **
-        GR.pts_to lr #one_half (vq + 1) **
-        pts_to x (v + 1)
-    {
+      : incr_f x
+        (fun v -> contributions left right 'i v)
+        (fun vq -> GR.pts_to lr #0.5R vq)
+      = v vq
+    { 
       unfold contributions;
       if b
       {
         with _p _v. rewrite (GR.pts_to lr #_p _v) as (GR.pts_to left #_p _v);
         GR.gather left;
         GR.write left (vq + 1);
-        GR.share left;
+        GR.share left;      
         with _p _v. rewrite (GR.pts_to left #_p _v) as (GR.pts_to lr #_p _v);
         fold (contributions left right 'i (v + 1));
       }
@@ -214,22 +246,24 @@ ensures pts_to x ('i + 2)
         with _p _v. rewrite (GR.pts_to lr #_p _v) as (GR.pts_to right #_p _v);
         GR.gather right;
         GR.write right (vq + 1);
-        GR.share right;
+        GR.share right;      
         with _p _v. rewrite (GR.pts_to right #_p _v) as (GR.pts_to lr #_p _v);
         fold (contributions left right 'i (v + 1));
       }
     };
-
-    par (fun _ -> incr x lock (step left true))
-        (fun _ -> incr x lock (step right false));
-
-    L.acquire lock; //we leak the lock here, but we can do better, below
-    unfold contributions;
+    L.share lock;
+    par (fun _ -> incr x #0.5R lock (step left true) #0)
+        (fun _ -> incr x #0.5R lock (step right false) #0);
+    L.gather lock;
+    L.acquire lock;
+    L.free lock;
+    unfold (contributions left right 'i);
     GR.gather left;
     GR.gather right;
     GR.free left;
     GR.free right;
 }
+//end add2_v2$
 
 //Note, rather than using two ghost references and duplicating code
 //monoids and use just a single piece of ghost state. But, that's for another
@@ -244,100 +278,108 @@ ensures pts_to x ('i + 2)
 //atomic_primitives$
 assume
 val atomic_read (r:ref int) (#p:_) (#i:erased int)
-  : stt_atomic int emp_inames
+  : stt_atomic int emp_inames 
     (pts_to r #p i)
     (fun v -> pts_to r #p i ** pure (reveal i == v))
 
 assume
 val cas (r:ref int) (u v:int) (#i:erased int)
-  : stt_atomic bool emp_inames
+  : stt_atomic bool emp_inames 
     (pts_to r i)
     (fun b ->
-      cond b (pts_to r v ** pure (reveal i == u))
+      cond b (pts_to r v ** pure (reveal i == u)) 
              (pts_to r i))
-//atomic_primitives$
+//end atomic_primitives$
 
 //This provides a way to allocate an invariant
 //and then discard it
 module C = Pulse.Lib.CancellableInvariant
 
+//incr_atomic_spec$
 fn incr_atomic
         (x: ref int)
         (#p:perm)
-        (#t:erased C.token)
-        (#refine #aspec: int -> vprop)
-        (l:inv (C.cancellable t (exists* v. pts_to x v ** refine v)))
-        (f: (v:int -> vq:int -> stt_ghost unit emp_inames
-                  (refine v ** aspec vq ** pts_to x (v + 1))
-                  (fun _ -> refine (v + 1) ** aspec (vq + 1) ** pts_to x (v + 1))))
-requires aspec 'i ** C.active p t
-ensures aspec ('i + 1) ** C.active p t
+        (#refine #aspec: int -> slprop)
+        (c:C.cinv)
+        (f: incr_f x refine aspec)
+requires inv (C.iname_of c) (C.cinv_vp c (exists* v. pts_to x v ** refine v)) ** aspec 'i ** C.active c p
+ensures inv (C.iname_of c) (C.cinv_vp c (exists* v. pts_to x v ** refine v)) ** aspec ('i + 1) ** C.active c p
+//end incr_atomic_spec$
 //incr_atomic_body$
 {
   //incr_atomic_body_read$
   atomic
   fn read ()
-  requires C.active p t
+  requires inv (C.iname_of c) (C.cinv_vp c (exists* v. pts_to x v ** refine v)) ** C.active c p ** later_credit 1
+  opens [C.iname_of c]
   returns v:int
-  ensures C.active p t
-  opens (add_inv emp_inames l)
+  ensures inv (C.iname_of c) (C.cinv_vp c (exists* v. pts_to x v ** refine v)) ** C.active c p
   {
-    with_invariants l
-    {
-        C.take _;
+    with_invariants_a int emp_inames (C.iname_of c) (C.cinv_vp c (exists* v. pts_to x v ** refine v))
+      (C.active c p) (fun _ -> C.active c p) fn _ {
+    // with_invariants (C.iname_of c) (C)
+    // {
+    //     later_elim _;
+        C.unpack_cinv_vp #p c;
         let v = atomic_read x;
-        C.restore (exists* v. pts_to x v ** refine v);
+        C.pack_cinv_vp #(exists* v. pts_to x v ** refine v) c;
+        // later_intro (C.cinv_vp c (exists* v. pts_to x v ** refine v));
         v
     }
   };
-  //incr_atomic_body_read$
+  //end incr_atomic_body_read$
   //incr_atomic_body_loop$
   let mut continue = true;
   fold (cond true (aspec 'i) (aspec ('i + 1)));
-  while (
-    with _b. _;
-    let b = !continue;
-    rewrite each _b as b;
-    b
-  )
-  invariant b.
+  while (!continue)
+  invariant exists* b.
+    inv (C.iname_of c) (C.cinv_vp c (exists* v. pts_to x v ** refine v)) **
     pts_to continue b **
-    C.active p t **
+    C.active c p **
     cond b (aspec 'i) (aspec ('i + 1))
   {
+    rewrite each (!continue) as true; // FIXME: rewrites_to goes in the wrong direction
+    later_credit_buy 1;
     let v = read ();
     let next =
-      with_invariants l
-      returns b1:bool
-      ensures cond b1 (aspec 'i) (aspec ('i + 1))
+      with_invariants bool emp_inames
+        (C.iname_of c) (C.cinv_vp c (exists* v. pts_to x v ** refine v))
+        (C.active c p ** pts_to continue true **
+          cond (!continue) (aspec 'i) (aspec ('i + 1)))
+        (fun b1 -> cond b1 (aspec 'i) (aspec ('i + 1))
           ** pts_to continue true
-          ** C.active p t
-      {
-        C.take _;
+          ** C.active c p)
+      fn _ {
+        C.unpack_cinv_vp c;
+        unfold cond;
+        with vv. assert x |-> vv;
         let b = cas x v (v + 1);
         if b
-        {
-          elim_cond_true b _ _;
-          elim_cond_true true _ _;
-          f _ _;
-          intro_cond_false (aspec 'i) (aspec ('i + 1));
-          C.restore (exists* v. pts_to x v ** refine v);
+        { 
+          unfold cond;
+          f vv 'i;
+          C.pack_cinv_vp #(exists* v. pts_to x v ** refine v) c;
+          fold (cond false (aspec 'i) (aspec ('i + 1)));
           false
         }
         else
         {
-          with p q. rewrite (cond b p q) as q;
-          C.restore (exists* v. pts_to x v ** refine v);
+          unfold cond;
+          C.pack_cinv_vp #(exists* v. pts_to x v ** refine v) c;
+          fold (cond true (aspec 'i) (aspec ('i + 1)));
           true
         }
       };
     continue := next
   };
-  //incr_atomic_body_loop$
+  //end incr_atomic_body_loop$
+  rewrite each (!continue) as false; // FIXME: rewrites_to goes in the wrong direction
   unfold cond;
 }
+//end incr_atomic_body$
 
 
+//add2_v3$
 fn add2_v3 (x: ref int)
 requires pts_to x 'i
 ensures pts_to x ('i + 2)
@@ -347,34 +389,27 @@ ensures pts_to x ('i + 2)
     GR.share left;
     GR.share right;
     fold (contributions left right 'i 'i);
-    let tok = C.create2 (
+    let c = C.new_cancellable_invariant (
       exists* (v:int).
           pts_to x v **
           contributions left right 'i v
     );
-    C.share tok;
-    let inv = new_invariant (C.cancellable tok _);
     ghost
     fn step
         (lr:GR.ref int)
         (b:bool { if b then lr == left else lr == right })
-        (v vq:int)
-      requires
-        contributions left right 'i v **
-        GR.pts_to lr #one_half vq **
-        pts_to x (v + 1)
-      ensures
-        contributions left right 'i (v + 1) **
-        GR.pts_to lr #one_half (vq + 1) **
-        pts_to x (v + 1)
-    {
+      : incr_f x
+        (fun v -> contributions left right 'i v)
+        (fun vq -> GR.pts_to lr #0.5R vq)
+      = v vq
+    { 
       unfold contributions;
       if b
       {
         with _p _v. rewrite (GR.pts_to lr #_p _v) as (GR.pts_to left #_p _v);
         GR.gather left;
         GR.write left (vq + 1);
-        GR.share left;
+        GR.share left;      
         with _p _v. rewrite (GR.pts_to left #_p _v) as (GR.pts_to lr #_p _v);
         fold (contributions left right 'i (v + 1));
       }
@@ -383,21 +418,330 @@ ensures pts_to x ('i + 2)
         with _p _v. rewrite (GR.pts_to lr #_p _v) as (GR.pts_to right #_p _v);
         GR.gather right;
         GR.write right (vq + 1);
-        GR.share right;
+        GR.share right;      
         with _p _v. rewrite (GR.pts_to right #_p _v) as (GR.pts_to lr #_p _v);
         fold (contributions left right 'i (v + 1));
       }
     };
-
-    par (fun _ -> incr_atomic x inv (step left true))
-        (fun _ -> incr_atomic x inv (step right false));
-
-    C.gather tok;
-    C.cancel_inv inv;
+    C.share c;
+    with pred. assert (inv (C.iname_of c) (C.cinv_vp c (exists* v. pts_to x v ** pred v)));
+    dup_inv (C.iname_of c) (C.cinv_vp c (exists* v. pts_to x v ** pred v));
+    par (fun _ -> incr_atomic x #0.5R c (step left true) #0)
+        (fun _ -> incr_atomic x #0.5R c (step right false) #0);
+    
+    C.gather c;
+    later_credit_buy 1;
+    C.cancel c;
     unfold contributions;
     GR.gather left;
     GR.gather right;
     GR.free left;
     GR.free right;
+    drop_ (inv _ _)
+}
+//end add2_v3$
 
+
+///////////////////////////////////////////////////////////////////////////////
+// Using single ghost state with a pcm to manage the views of the two threads
+// We pick product of two fractional permission PCMs as the ghost state
+///////////////////////////////////////////////////////////////////////////////
+
+open FStar.PCM
+
+module G = FStar.Ghost
+module Prod = Pulse.Lib.PCM.Product
+module Frac = Pulse.Lib.PCM.Fraction
+
+type ghost_st : Type0 = Frac.fractional int & Frac.fractional int
+
+let pcm : pcm ghost_st = Prod.pcm_prod Frac.pcm_frac Frac.pcm_frac
+
+let with_p (n:int) (p:perm) : Frac.fractional int = Some (n, p)
+let full (n:int) : Frac.fractional int = Some (n, 1.0R)
+let half (n:int) : Frac.fractional int = Some (n, 0.5R)
+
+let fp_upd_t1
+  (t1_old:G.erased int) 
+  (t1_new:int)
+  (t2:int)
+  (p2:perm)
+  
+  : frame_preserving_upd pcm (full t1_old, with_p t2 p2) (full t1_new, with_p t2 p2) =
+  
+  Prod.mk_frame_preserving_upd_fst
+    #_
+    #_
+    #Frac.pcm_frac
+    #Frac.pcm_frac
+    _
+    _
+    (with_p t2 p2)
+    (Frac.mk_frame_preserving_upd t1_old t1_new)
+
+let fp_upd_t2
+  (t1:int)
+  (p1:perm)
+  (t2_old:G.erased int) 
+  (t2_new:int)
+  
+  : frame_preserving_upd pcm (with_p t1 p1, full t2_old) (with_p t1 p1, full t2_new) =
+  
+  Prod.mk_frame_preserving_upd_snd
+    #_
+    #_
+    #Frac.pcm_frac
+    #Frac.pcm_frac
+    (with_p t1 p1)
+    _
+    _
+    (Frac.mk_frame_preserving_upd t2_old t2_new)
+
+module GPR = Pulse.Lib.GhostPCMReference
+
+ghost
+fn share (r:GPR.gref pcm) (#n1 #n2:int)
+  requires GPR.pts_to r (full n1, full n2)
+  ensures GPR.pts_to r (half n1, None) **
+          GPR.pts_to r (None, half n2) **
+          GPR.pts_to r (half n1, half n2)
+{
+  rewrite (GPR.pts_to r (full n1, full n2)) as
+          (GPR.pts_to r ((half n1, None) `op pcm` (half n1, full n2)));
+  GPR.share r (half n1, None) (half n1, full n2);
+  rewrite (GPR.pts_to r (half n1, full n2)) as
+          (GPR.pts_to r ((None, half n2) `op pcm` (half n1, half n2)));
+  GPR.share r (None, half n2) (half n1, half n2)
+}
+
+
+
+ghost
+fn gather (r:GPR.gref pcm) (#n1 #n2:int) (#v1 #v2:int)
+  requires GPR.pts_to r (half n1, None) **
+           GPR.pts_to r (None, half n2) **
+           GPR.pts_to r (half v1, half v2)
+  returns _:squash (v1 == n1 /\ v2 == n2)
+  ensures GPR.pts_to r (full n1, full n2)
+
+{
+  GPR.gather r (None, half n2) (half v1, half v2);
+  rewrite (GPR.pts_to r ((None, half n2) `op pcm` (half v1, half v2))) as
+          (GPR.pts_to r (half v1, full n2));
+  GPR.gather r (half n1, None) (half v1, full n2);
+  rewrite (GPR.pts_to r ((half n1, None) `op pcm` (half v1, full n2))) as
+          (GPR.pts_to r (full n1, full n2))
+}
+
+
+let lock_inv_ghost (ghost_r:GPR.gref pcm) (n:int) : timeless_slprop =
+  exists* n1 n2. GPR.pts_to ghost_r (half n1, half n2) **
+                 pure (n == n1 + n2)
+
+let lock_inv_pcm (r:ref int) (ghost_r:GPR.gref pcm) : timeless_slprop =
+  exists* n. pts_to r n ** lock_inv_ghost ghost_r n
+
+let t1_perm (ghost_r:GPR.gref pcm) (n:int) (t1:bool) =
+  if t1
+  then GPR.pts_to ghost_r (half n, None)
+  else GPR.pts_to ghost_r (None, half n)
+
+let add_one (n:int) : int = n + 1
+
+//
+// Lock, increment the reference, and
+//  update the ghost state's first component if t1 = true, else the second
+// 
+
+fn incr_pcm_t (r:ref int) (ghost_r:GPR.gref pcm) (l:L.lock) (t1:bool) (#n:int)
+  requires L.lock_alive l #0.5R (lock_inv_pcm r ghost_r) **
+           t1_perm ghost_r n t1
+  ensures L.lock_alive l #0.5R (lock_inv_pcm r ghost_r) **
+          t1_perm ghost_r (add_one n) t1
+{
+  L.acquire l;
+  unfold lock_inv_pcm; with n'. _;
+  unfold lock_inv_ghost; with n1 n2. _;
+  let v = !r;
+  r := v + 1;
+  if t1 {
+    rewrite (t1_perm ghost_r n t1) as
+            (GPR.pts_to ghost_r (half n, None));
+    GPR.gather ghost_r (half n, None) (half n1, half n2);
+    rewrite (GPR.pts_to ghost_r ((half n, None) `op pcm` (half n1, half n2))) as
+            (GPR.pts_to ghost_r (full n1, half n2));
+    GPR.write ghost_r
+      (full n1, half n2)
+      (full (add_one n1), half n2)
+      (fp_upd_t1 n1 (add_one n1) n2 0.5R);
+    rewrite (GPR.pts_to ghost_r (full (add_one n1), half n2)) as
+            (GPR.pts_to ghost_r ((half (add_one n1), half n2) `op pcm` (half (add_one n1), None)));
+    GPR.share ghost_r (half (add_one n1), half n2) (half (add_one n1), None);
+    fold lock_inv_ghost ghost_r (!r);
+    fold lock_inv_pcm r;
+    L.release l;
+    fold (t1_perm ghost_r (add_one n) true);
+  } else {
+    rewrite (t1_perm ghost_r n t1) as
+            (GPR.pts_to ghost_r (None, half n));
+    GPR.gather ghost_r (None, half n) (half n1, half n2);
+    rewrite (GPR.pts_to ghost_r ((None, half n2) `op pcm` (half n1, half n2))) as
+            (GPR.pts_to ghost_r (half n1, full n2));
+    GPR.write ghost_r
+      (half n1, full n2)
+      (half n1, full (add_one n2))
+      (fp_upd_t2 n1 0.5R n2 (add_one n2));
+    rewrite (GPR.pts_to ghost_r (half n1, full (add_one n2))) as
+            (GPR.pts_to ghost_r ((half n1, half (add_one n2)) `op pcm` (None, half (add_one n2))));
+    GPR.share ghost_r (half n1, half (add_one n2)) (None, half (add_one n2));
+    fold lock_inv_ghost ghost_r (!r);
+    fold lock_inv_pcm;
+    L.release l;
+    fold (t1_perm ghost_r (add_one n) false)
+  }
+}
+
+
+fn incr_pcm (r:ref int) (#n:erased int)
+  requires pts_to r 0
+  ensures pts_to r 2
+{
+  let ghost_r = GPR.alloc #_ #pcm (G.hide (full 0, full 0));
+  with _v. rewrite (GPR.pts_to ghost_r (G.reveal (G.hide _v))) as
+                   (GPR.pts_to ghost_r _v);
+  share ghost_r;
+  fold lock_inv_ghost;
+  fold lock_inv_pcm;
+
+  rewrite (GPR.pts_to ghost_r (half 0, None)) as
+          (t1_perm ghost_r 0 true);
+  rewrite (GPR.pts_to ghost_r (None, half 0)) as
+          (t1_perm ghost_r 0 false);
+
+  let l = L.new_lock (lock_inv_pcm r ghost_r);
+  
+  L.share l;
+
+  par #(requires L.lock_alive l #0.5R (lock_inv_pcm r ghost_r) **
+             t1_perm ghost_r 0 true)
+      #(requires L.lock_alive l #0.5R (lock_inv_pcm r ghost_r) **
+             t1_perm ghost_r 0 false)
+      #(ensures L.lock_alive l #0.5R (lock_inv_pcm r ghost_r) **
+            t1_perm ghost_r (add_one 0) true)
+      #(ensures L.lock_alive l #0.5R (lock_inv_pcm r ghost_r) **
+            t1_perm ghost_r (add_one 0) false)
+    fn _ { incr_pcm_t r ghost_r l true }
+    fn _ { incr_pcm_t r ghost_r l false };
+
+  L.gather l;
+  L.acquire l;
+  unfold lock_inv_pcm;
+  unfold lock_inv_ghost;
+  unfold (t1_perm ghost_r (add_one 0) true);
+  unfold (t1_perm ghost_r (add_one 0) false);
+  gather ghost_r;
+  L.free l;
+  drop_ (GPR.pts_to ghost_r _)
+}
+
+
+//////////////////////////////////////////////////////////////////////////////////////////
+// Passing ghost steps to incr, a similar style to Bart Jacobs & Frank Piessens POPL '11
+//////////////////////////////////////////////////////////////////////////////////////////
+
+
+fn incr_pcm_t_abstract (r:ref int) (l:L.lock)
+  (#ghost_inv:int -> slprop)
+  (#ghost_pre:slprop)
+  (#ghost_post:slprop)
+  (ghost_steps:
+     (v:int ->
+      stt_ghost unit emp_inames
+        (ghost_pre ** ghost_inv v)
+        (fun _ -> ghost_post ** ghost_inv (v + 1))))
+  requires L.lock_alive l #0.5R (exists* v. pts_to r v ** ghost_inv v) **
+           ghost_pre
+  ensures L.lock_alive l #0.5R (exists* v. pts_to r v ** ghost_inv v) **
+          ghost_post
+{
+  L.acquire l;
+  let v = !r;
+  r := v + 1;
+  ghost_steps v;
+  L.release #(exists* v. pts_to r v ** ghost_inv v) l
+}
+
+
+
+fn incr_pcm_abstract (r:ref int)
+  requires pts_to r 0
+  ensures pts_to r 2
+{
+  let ghost_r = GPR.alloc #_ #pcm (G.hide (full 0, full 0));
+
+  ghost
+  fn t1 (v:int)
+    requires GPR.pts_to ghost_r (half 0, None) ** lock_inv_ghost ghost_r v
+    ensures GPR.pts_to ghost_r (half (add_one  0), None) ** lock_inv_ghost ghost_r (v + 1)
+  {
+    unfold lock_inv_ghost;
+    with n1 n2. assert (GPR.pts_to ghost_r (half n1, half n2));
+    GPR.gather ghost_r (half 0, None) (half n1, half n2);
+    rewrite (GPR.pts_to ghost_r ((half 0, None) `op pcm` (half n1, half n2))) as
+            (GPR.pts_to ghost_r (full n1, half n2));
+    GPR.write ghost_r
+      (full n1, half n2)
+      (full (add_one n1), half n2)
+      (fp_upd_t1 n1 (add_one n1) n2 0.5R);
+    rewrite (GPR.pts_to ghost_r (full (add_one n1), half n2)) as
+            (GPR.pts_to ghost_r ((half (add_one n1), half n2) `op pcm` (half (add_one n1), None)));
+    GPR.share ghost_r (half (add_one n1), half n2) (half (add_one n1), None);
+    fold ((lock_inv_ghost ghost_r) (v + 1))
+  };
+
+  ghost
+  fn t2 (v:int)
+    requires GPR.pts_to ghost_r (None, half 0) ** lock_inv_ghost ghost_r v
+    ensures GPR.pts_to ghost_r (None, half (add_one  0)) ** lock_inv_ghost ghost_r (v +1)
+  {
+    unfold lock_inv_ghost;
+    with n1 n2. assert (GPR.pts_to ghost_r (half n1, half n2));
+    GPR.gather ghost_r (None, half 0) (half n1, half n2);
+    rewrite (GPR.pts_to ghost_r ((None, half n2) `op pcm` (half n1, half n2))) as
+            (GPR.pts_to ghost_r (half n1, full n2));
+    GPR.write ghost_r
+      (half n1, full n2)
+      (half n1, full (add_one n2))
+      (fp_upd_t2 n1 0.5R n2 (add_one n2));
+    rewrite (GPR.pts_to ghost_r (half n1, full (add_one n2))) as
+            (GPR.pts_to ghost_r ((half n1, half (add_one n2)) `op pcm` (None, half (add_one n2))));
+    GPR.share ghost_r (half n1, half (add_one n2)) (None, half (add_one n2));
+    fold ((lock_inv_ghost ghost_r) (v + 1))
+  };
+
+  with _v. rewrite (GPR.pts_to ghost_r (G.reveal (G.hide _v))) as
+                   (GPR.pts_to ghost_r _v);
+  share ghost_r;
+  fold lock_inv_ghost;
+  let l = L.new_lock (exists* v. pts_to r v ** lock_inv_ghost ghost_r v);
+  L.share l;
+
+  par
+    #(requires L.lock_alive l #0.5R (exists* v. pts_to r v ** lock_inv_ghost ghost_r v) **
+             GPR.pts_to ghost_r (half 0, None))
+    #(requires L.lock_alive l #0.5R (exists* v. pts_to r v ** lock_inv_ghost ghost_r v) **
+             GPR.pts_to ghost_r (None, half 0))
+    #(ensures L.lock_alive l #0.5R (exists* v. pts_to r v ** lock_inv_ghost ghost_r v) **
+            GPR.pts_to ghost_r (half (add_one 0), None))
+    #(ensures L.lock_alive l #0.5R (exists* v. pts_to r v ** lock_inv_ghost ghost_r v) **
+            GPR.pts_to ghost_r (None, half (add_one 0)))
+    fn _ { incr_pcm_t_abstract r l t1 }
+    fn _ { incr_pcm_t_abstract r l t2 };
+
+  L.gather l;
+  L.acquire l;
+  unfold lock_inv_ghost;
+  gather ghost_r;
+  L.free l;
+  drop_ (GPR.pts_to ghost_r _)
 }
