src/tutorial/exercises/PulseTutorialExercises.SpinLock2.fst
@@ -3,24 +3,23 @@
    ensuring that a lock cannot be double-released *)
 module PulseTutorialExercises.SpinLock2
 #lang-pulse
-open Pulse
-module Box = Pulse.Lib.Box
+open Pulse.Lib.Pervasives
 module U32 = FStar.UInt32
 module GR = Pulse.Lib.GhostReference
 
 //lock$
-let maybe (b:bool) (p:vprop) =
+let maybe (b:bool) (p:slprop) =
     if b then p else emp
 
-let lock_inv (r:ref U32.t) (gr:GR.ref U32.t) (p:vprop) =
-  exists* v perm.
+let lock_inv (r:ref U32.t) (gr:GR.ref U32.t) (p:slprop) =
+  exists* v perm. 
     pts_to r v **
     GR.pts_to gr #perm v **
     maybe (v = 0ul) p **
     pure (if v=0ul then perm == full_perm else perm == one_half)
 
 noeq
-type lock (p:vprop) = {
+type lock (p:slprop) = {
   r:ref U32.t;
   gr:GR.ref U32.t;
   i:inv (lock_inv r gr p);
@@ -29,13 +28,16 @@ type lock (p:vprop) = {
 
 let locked #p (l:lock p) = GR.pts_to l.gr #one_half 1ul
 
-fn new_lock (p:vprop)
+
+fn new_lock (p:slprop)
 requires p
 returns l:lock p
 ensures emp
 {
   admit()
 }
+
+
 
 
 fn rec acquire #p (l:lock p)
@@ -45,9 +47,12 @@ ensures p ** locked l
   admit()
 }
 
+
+
 fn release #p (l:lock p)
 requires p ** locked l
 ensures emp
 {
   admit()
 }
+
