src/tutorial/solutions/PulseTutorialSolutions.SpinLock3.fst
@@ -1,26 +1,26 @@
 module PulseTutorialSolutions.SpinLock3
 #lang-pulse
-open Pulse
+open Pulse.Lib.Pervasives
 module Box = Pulse.Lib.Box
 module U32 = FStar.UInt32
 module GR = Pulse.Lib.GhostReference
 
 //lock$
-let maybe ([@@@equate_by_smt] b:bool) (p:vprop) =
+let maybe ([@@@equate_by_smt] b:bool) (p:slprop) =
     if b then p else emp
 
-let core_lock_inv (r:Box.box U32.t) (p:vprop) =
+let core_lock_inv (r:Box.box U32.t) (p:slprop) = 
   exists* v.
       Box.pts_to r v **
       maybe (v = 0ul) p
 
-let lock_inv (r:Box.box U32.t) (live:GR.ref bool) (p:vprop) =
-  exists* b.
+let lock_inv (r:Box.box U32.t) (live:GR.ref bool) (p:slprop) =
+  exists* b. 
     GR.pts_to live #one_half b **
     maybe b (core_lock_inv r p)
 
 noeq
-type lock (p:vprop) = {
+type lock (p:slprop) = {
   r:Box.box U32.t;
   live:GR.ref bool;
   i:inv (lock_inv r live p);
@@ -29,6 +29,7 @@ type lock (p:vprop) = {
 let lock_live #p (l:lock p) (#[default_arg (`full_perm)] perm:perm) =
     GR.pts_to l.live #(half_perm perm) true
 //lock$
+
 
 fn new_lock ()
 requires p
@@ -50,11 +51,13 @@ ensures lock_live l
 }
 
 
+
+
 fn free_lock #p (l:lock p)
-requires lock_live l
+requires lock_live l 
 ensures emp
 {
-  with_invariants l.i
+  with_invariants l.i 
   returns _:unit
   ensures core_lock_inv l.r p
   {
@@ -75,6 +78,8 @@ ensures emp
   drop_ (maybe _ _); //leaks p; see previous exercise on how to prevent this
 }
 
+
+
 ghost
 fn share #p #q (l:lock p)
 requires lock_live l #q
@@ -86,11 +91,13 @@ ensures lock_live l #(half_perm q) ** lock_live l #(half_perm q)
   fold (lock_live l #(half_perm q));
 }
 
+
 let sum_halves (x y:perm)
  : Lemma (ensures sum_perm (half_perm x) (half_perm y) == half_perm (sum_perm x y))
          [SMTPat (sum_perm (half_perm x) (half_perm y))]
  = let open FStar.Real in
    assert (forall (x y:FStar.Real.real). ( x /. 2.0R ) +. (y /. 2.0R) == ((x +. y) /. 2.0R))
+
 
 ghost
 fn gather #p #q1 #q2 (l:lock p)
@@ -103,17 +110,22 @@ ensures lock_live l #(sum_perm q1 q2)
   fold (lock_live l #(sum_perm q1 q2));
 }
 
+
+
 fn acquire #p #q (l:lock p)
-requires lock_live l #q
+requires lock_live l #q 
 ensures p ** lock_live l #q
 {
     admit()
 }
 
+
+
 fn release #p #q (l:lock p)
-requires p ** lock_live l #q
+requires p ** lock_live l #q 
 ensures lock_live l #q
 {
     admit()
 }
+
 
