src/tutorial/PulseTutorial.AtomicsAndInvariants.fst
@@ -1,107 +1,152 @@
+(*
+   Copyright 2023 Microsoft Research
+
+   Licensed under the Apache License, Version 2.0 (the "License");
+   you may not use this file except in compliance with the License.
+   You may obtain a copy of the License at
+
+       http://www.apache.org/licenses/LICENSE-2.0
+
+   Unless required by applicable law or agreed to in writing, software
+   distributed under the License is distributed on an "AS IS" BASIS,
+   WITHOUT WARRANTIES OR CONDITIONS OF ANY KIND, either express or implied.
+   See the License for the specific language governing permissions and
+   limitations under the License.
+*)
+
 module PulseTutorial.AtomicsAndInvariants
 #lang-pulse
-open Pulse
+open Pulse.Lib.Pervasives
+module T = FStar.Tactics
 module U32 = FStar.UInt32
 
 //owns$
-let owns (x:ref U32.t) = exists* v. pts_to x v
-//owns$
+let owns (x:ref U32.t) : timeless_slprop = exists* v. pts_to x v
+//end owns$
 
+//owns_timeless$
+let owns_timeless (x:ref U32.t)
+: squash (timeless (owns x))
+by T.(norm [delta_only [`%owns; `%auto_squash]]; 
+      mapply (`FStar.Squash.return_squash);
+      mapply (`timeless_exists))
+= ()
+//end owns_timeless$
+
+//create_invariant$
+ghost
 fn create_invariant (r:ref U32.t) (v:erased U32.t)
 requires pts_to r v
-returns i:inv (owns r)
-ensures emp
+returns i:iname
+ensures inv i (owns r)
 {
     fold owns;
     new_invariant (owns r)
 }
+//end create_invariant$
 
-let singleton #p (i:inv p) = add_inv emp_inames i
-
+//update_ref_atomic$
 atomic
-fn update_ref_atomic (r:ref U32.t) (i:inv (owns r)) (v:U32.t)
-requires emp
-ensures emp
-opens (singleton i)
+fn update_ref_atomic (r:ref U32.t) (i:iname) (v:U32.t)
+requires inv i (owns r) ** later_credit 1
+ensures inv i (owns r)
+opens [i]
 {
-  with_invariants i {    //owns r
+  with_invariants_a unit emp_inames i (owns r) emp (fun _ -> emp)
+  fn _ { // owns r
      unfold owns;        //ghost step;  exists* u. pts_to r u
      write_atomic r v;   //atomic step; pts_to r v
      fold owns;          //ghost step;  owns r
-  }
+  } // inv i (owns r)
 }
+//end update_ref_atomic$
 
+[@@allow_ambiguous]
 ghost
-fn pts_to_dup_impossible #a (x:ref a)
+fn pts_to_dup_impossible u#a (#a: Type u#a) (x:ref a)
 requires pts_to x 'v ** pts_to x 'u
 ensures  pts_to x 'v ** pts_to x 'u ** pure False
 {
     gather x;
     pts_to_perm_bound x;
-    share x;
+    share x;    
 }
 
+
 //double_open_bad$
-[@@expect_failure]
-fn double_open_bad (r:ref U32.t) (i:inv (owns r))
-requires emp
+[@@expect_failure [19]]
+fn double_open_bad (r:ref U32.t) (i:iname)
+requires inv i (owns r)
 ensures pure False
 {
-    with_invariants i {
-      with_invariants i {
-        unfold owns;
-        unfold owns;
-        pts_to_dup_impossible r;
-        fold owns;
-        fold owns
-      }
-    }
+  dup (inv i (owns r)) ();
+  later_credit_buy 1;
+  with_invariants unit emp_inames i (owns r) (inv i (owns r) ** later_credit 1) (fun _ -> pure False) fn _ {
+    with_invariants_a unit emp_inames i (owns r) (owns r) (fun _ -> pure False) fn _ {
+      unfold owns; with v. _;
+      unfold owns; with u. _;
+      pts_to_dup_impossible r;
+      drop_ (r |-> u);
+      fold owns r;
+    };
+    rewrite inv i (owns r) as owns r;
+  };
+  drop_ (inv i (owns r));
 }
-//double_open_bad$
+//end double_open_bad$
 
-
-fn update_ref (r:ref U32.t) (i:inv (owns r)) (v:U32.t)
-requires emp
-ensures emp
-{
-  with_invariants i {    //owns r
-     unfold owns;        //ghost step;  exists* u. pts_to r u
-     write_atomic r v;   //atomic step; pts_to r v
-     fold owns;          //ghost step;  owns r
-  }
+//update_ref$
+fn update_ref (r:ref U32.t) (i:iname) (v:U32.t)
+requires inv i (owns r)
+ensures inv i (owns r)
+{                    
+  later_credit_buy 1;
+  update_ref_atomic r i v;
 }
+//end update_ref$
 
 //update_ref_fail$
-[@@expect_failure]
-fn update_ref_fail (r:ref U32.t) (i:inv (owns r)) (v:U32.t)
-requires emp
-ensures emp
+[@@expect_failure [228]]
+fn update_ref_fail (r:ref U32.t) (i:iname) (v:U32.t)
+requires inv i (owns r)
+ensures inv i (owns r)
 {
-  with_invariants i {
+  with_invariants unit emp_inames i (owns r) emp (fun _ -> emp) fn _ {
     unfold owns;
     r := v; //not atomic
     fold owns;
   }
 }
-//update_ref_fail$
+//end update_ref_fail$
 
+let readable (r:ref U32.t) : timeless_slprop  = exists* p v. pts_to r #p v
 
-
-let readable (r:ref U32.t) = exists* p v. pts_to r #p v
-
-atomic
-fn split_readable (r:ref U32.t) (i:inv (readable r))
-requires emp
-ensures readable r
-opens (singleton i)
+ghost
+fn intro_readable (r:ref U32.t) (p:perm) (v:U32.t)
+  requires pts_to r #p v
+  ensures  readable r
 {
-    with_invariants i {
-        unfold readable;
-        share r;
-        fold readable;
-        fold readable;
-    };
+  fold readable
 }
 
 
-
+//split_readable$
+ghost
+fn split_readable (r:ref U32.t) (i:iname)
+requires inv i (readable r)
+requires later_credit 1
+ensures inv i (readable r) ** readable r
+opens [i]
+{
+  with_invariants_g unit emp_inames i (readable r) emp (fun _ -> readable r) fn _ {
+        unfold readable;
+        with p v. assert (pts_to r #p v);
+        share r;
+        (* just folding readable would now be ambiguous, need the explicit intro. *)
+        // fold readable;
+        // fold readable;
+        intro_readable r (p /. 2.0R) _;
+        intro_readable r (p /. 2.0R) _;
+    };
+}
+//end split_readable$
