src/tutorial/PulseTutorial.Loops.fst
@@ -16,60 +16,91 @@
 
 module PulseTutorial.Loops
 #lang-pulse
-open Pulse
+open Pulse.Lib.Pervasives
+module R = Pulse.Lib.Reference
 
+//count_down$
 fn count_down (x:ref nat)
-requires pts_to x 'v
-ensures pts_to x 0
+requires R.pts_to x 'v
+ensures  R.pts_to x 0
 {
     let mut keep_going = true;
     while (
         !keep_going
     )
-    invariant b.
-      exists* v.
+    invariant
+      exists* (b:bool) (v:nat).
         pts_to keep_going b **
         pts_to x v **
-        pure (b == false ==> v == 0)
+        pure (not b  ==> v == 0)
     {
         let n = !x;
-        if (n = 0)
+        if (n = 0) 
         {
             keep_going := false;
-        }
+        } 
         else
         {
             x := n - 1;
         }
     }
 }
+//end count_down$
 
-fn count_down2 (x:ref nat)
-requires pts_to x 'v
-ensures pts_to x 0
+fn count_down2 (x:ref nat) (#v:erased nat)
+requires R.pts_to x v
+ensures  R.pts_to x 0
+{
+    let mut keep_going = true;
+    let mut decr : nat = 1;
+    while (
+        !keep_going
+    )
+    invariant
+      exists* (b:bool) (v:nat).
+        pts_to keep_going b **
+        pts_to x v **
+        pure (not b ==> v == 0)
+    {   let n = !x;
+        if (n = 0) 
+        {
+            keep_going := false;
+        } 
+        else
+        {
+            x := n - !decr;
+        }
+    }
+}
+
+//count_down3$
+fn count_down3 (x:ref nat)
+requires R.pts_to x 'v
+ensures  R.pts_to x 0
 {
     while (
         let n = !x;
         if (n = 0)
         {
             false
-        }
+        } 
         else
         {
             x := n - 1;
             true
         }
     )
-    invariant b.
-      exists* v.
-        pts_to x v **
-        pure (b == false ==> v == 0)
+    invariant
+      exists* (v:nat). pts_to x v
     { () }
 }
+//end count_down3$
 
+
+//count_down_loopy$
 fn count_down_loopy (x:ref nat)
-requires pts_to x 'v
-ensures pts_to x 0
+requires R.pts_to x 'v
+ensures  R.pts_to x 0
 {
     while (
         let n = !x;
@@ -83,14 +114,14 @@ ensures pts_to x 0
             true
         }
     )
-    invariant b.
-      exists* v.
-        pts_to x v **
-        pure (b == false ==> v == 0)
+    invariant exists* v. R.pts_to x v
     { () }
 }
+//end count_down_loopy$
+
 open FStar.Mul
 
+//multiply_by_repeated_addition$
 fn multiply_by_repeated_addition (x y:nat)
     requires emp
     returns z:nat
@@ -98,17 +129,13 @@ fn multiply_by_repeated_addition (x y:nat)
 {
     let mut ctr : nat = 0;
     let mut acc : nat = 0;
-    while (
-        let c = !ctr;
-        (c < x)
-    )
-    invariant b.
-    exists* c a.
-        pts_to ctr c **
-        pts_to acc a **
+    while ( (!ctr < x) )
+    invariant 
+    exists* (c a : nat).
+        R.pts_to ctr c **
+        R.pts_to acc a **
         pure (c <= x /\
-              a == (c * y) /\
-              b == (c < x))
+              a == (c * y))
     {
         let a = !acc;
         acc := a + y;
@@ -117,20 +144,29 @@ fn multiply_by_repeated_addition (x y:nat)
     };
     !acc
 }
+//end multiply_by_repeated_addition$
 
-//SNIPPET_START: sum$
+
+noextract
+//sum$
 let rec sum (n:nat)
 : nat
 = if n = 0 then 0 else n + sum (n - 1)
 
+#push-options "--z3rlimit 20"
+noextract
 let rec sum_lemma (n:nat)
 : Lemma (sum n == n * (n + 1) / 2)
 = if n = 0 then ()
   else sum_lemma (n - 1)
-//SNIPPET_END: sum$
+#pop-options
+//end sum$
 
-//SNIPPET_START: isum$
+
+//isum$
 #push-options "--z3cliopt 'smt.arith.nl=false'"
+noextract
+
 fn isum (n:nat)
 requires emp
 returns z:nat
@@ -138,17 +174,13 @@ ensures pure ((n * (n + 1) / 2) == z)
 {
     let mut acc : nat = 0;
     let mut ctr : nat = 0;
-    while (
-        let c = !ctr;
-        (c < n)
-    )
-    invariant b.
-    exists* c a.
-        pts_to ctr c **
-        pts_to acc a **
+    while ( (!ctr < n ) )
+    invariant 
+    exists* (c a : nat).
+        R.pts_to ctr c **
+        R.pts_to acc a **
         pure (c <= n /\
-              a == sum c /\
-              b == (c < n))
+              a == sum c)
     {
         let a = !acc;
         let c = !ctr;
@@ -159,14 +191,17 @@ ensures pure ((n * (n + 1) / 2) == z)
     !acc;
 }
 #pop-options
-//SNIPPET_END: isum$
+//end isum$
 
+noextract
 //fib$
 let rec fib (n:nat) : nat =
   if n <= 1 then 1
   else fib (n - 1) + fib (n - 2)
-//fib$
+//end fib$
 
+noextract
+ //fib_rec$
 fn rec fib_rec (n:pos) (out:ref (nat & nat))
 requires
     pts_to out 'v
@@ -175,15 +210,15 @@ ensures
         pts_to out v **
         pure (
           fst v == fib (n - 1) /\
-          snd v == fib n
+          snd v == fib n 
         )
 {
-  if ((n = 1))
+  if (n = 1)
   {
     //type inference in Pulse doesn't work well here:
     //it picks (1, 1) to have type (int & int)
     //so we have to annotate
-    out := ((1 <: nat), (1 <: nat));
+    out := ((1 <: nat), (1 <: nat)); 
   }
   else
   {
@@ -192,7 +227,9 @@ ensures
     out := (snd v, fst v + snd v);
   }
 }
+//end fib_rec$
 
+//fib_loop$
 fn fib_loop (k:pos)
   requires emp
   returns r:nat
@@ -201,22 +238,17 @@ fn fib_loop (k:pos)
   let mut i : nat = 1;
   let mut j : nat = 1;
   let mut ctr : nat = 1;
-  while (
-    let c = !ctr;
-    (c < k)
-  )
-  invariant b .
-    exists* vi vj vctr.
-        pts_to i vi **
-        pts_to j vj **
-        pts_to ctr vctr **
+  while (!ctr < k)
+  invariant
+    exists* (vi vj vctr : nat).
+        R.pts_to i vi **
+        R.pts_to j vj **
+        R.pts_to ctr vctr **
         pure (
             1 <= vctr /\
             vctr <= k /\
             vi == fib (vctr - 1) /\
-            vj == fib vctr /\
-            b == (vctr < k)
-        )
+            vj == fib vctr) 
   {
       let vi = !i;
       let vj = !j;
@@ -227,9 +259,9 @@ fn fib_loop (k:pos)
   };
   !j
 }
+//end fib_loop$
 
-
-
+noextract
 let rec fib_mono (n:nat) (m:nat { m <= n})
   : Lemma
     (ensures fib m <= fib n)
@@ -240,7 +272,8 @@ open FStar.UInt32
 open Pulse.Lib.BoundedIntegers
 module U32 = FStar.UInt32
 
-
+noextract
+//fibonacci32$
 fn fibonacci32 (k:U32.t)
   requires pure (0ul < k /\ fib (v k) < pow2 32)
   returns r:U32.t
@@ -249,20 +282,16 @@ fn fibonacci32 (k:U32.t)
   let mut i = 1ul;
   let mut j = 1ul;
   let mut ctr = 1ul;
-  while (
-    let c = !ctr;
-    (c < k)
-  )
-  invariant b .
-    exists* vi vj vctr.
-     pts_to i vi **
-     pts_to j vj **
-     pts_to ctr vctr **
+  while (!ctr < k)
+  invariant
+    exists* vi vj vctr. 
+     R.pts_to i vi **
+     R.pts_to j vj **
+     R.pts_to ctr vctr **
      pure (1ul <= vctr /\
            vctr <= k /\
            fib (v (vctr - 1ul)) == v vi/\
-           fib (v vctr) == v vj /\
-           b == (vctr < k))
+           fib (v vctr) == v vj)
   {
      let vi = !i;
      let vj = !j;
@@ -274,3 +303,4 @@ fn fibonacci32 (k:U32.t)
   };
   !j
 }
+//end fibonacci32$
