src/tutorial/exercises/PulseTutorialExercises.Basics.fst
@@ -1,16 +1,19 @@
 module PulseTutorialExercises.Basics
 #lang-pulse
-open Pulse
+open Pulse.Lib.Pervasives
 
 let fstar_five : int = 5
+
 
 fn five ()
 requires emp
 returns n:int
 ensures pure (n == 5)
-{
+{ 
   fstar_five
 }
+
+
 
 fn incr (r:ref int) (#n:erased int) // since n is purely specificational, it is erased
   requires pts_to r n
@@ -20,6 +23,8 @@ fn incr (r:ref int) (#n:erased int) // since n is purely specificational, it is 
     r := x + 1
 }
 
+
+
 fn read (r:ref int) p (n:erased int) // any permission is ok for reading
 requires pts_to r #p n
 returns x:int
@@ -27,6 +32,8 @@ ensures pts_to r #p n ** pure (x == n)
 {
     !r
 }
+
+
 
 fn write (r:ref int) (n:erased int) // write requires full permission
   requires pts_to r #full_perm n
@@ -36,7 +43,9 @@ fn write (r:ref int) (n:erased int) // write requires full permission
     r := y
 }
 
+
 [@@ expect_failure] // fails
+
 fn write (r:ref int) p (n:erased int)
   requires pts_to r #p n
   ensures pts_to r #p n
@@ -44,6 +53,8 @@ fn write (r:ref int) p (n:erased int)
     let y = !r;
     r := y
 }
+
+
 
 fn incr2 (r1 r2:ref int)
   requires pts_to r1 'n1 ** pts_to r2 'n2
@@ -58,6 +69,8 @@ fn incr2 (r1 r2:ref int)
     // pts_to r1 (‘n1 + 1) ** pts_to r2 (‘n2 + 1)
 }
 
+
+
 fn incr_stack ()
   requires emp
   returns x:int
@@ -68,7 +81,9 @@ fn incr_stack ()
     !i  // explicit dereference, no need to free i, automatically reclaimed when the function returns
 }
 
+
 module Box = Pulse.Lib.Box
+
 fn incr_heap ()
   requires emp
   returns x:int
@@ -83,10 +98,13 @@ fn incr_heap ()
     x
 }
 
+
 //Exercise 1: Fill in the spec and implementation of swap
+
 fn swap #a (r1 r2:ref a)
 requires emp
 ensures emp
 {
     admit()
 }
+
