src/tutorial/exercises/PulseTutorialExercises.SumArray.fst
@@ -1,30 +1,35 @@
 module PulseTutorialExercises.SumArray
 #lang-pulse
-open Pulse
+open Pulse.Lib.Pervasives
 open Pulse.Lib.Array
 module SZ = FStar.SizeT
 open FStar.SizeT
 module R = Pulse.Lib.Reference
 open FStar.Seq
 
+
 fn read (arr:array int) (s:erased (seq int) { Seq.length s > 0 })
   requires pts_to arr s
   returns x:int
   ensures pts_to arr s ** pure (x == Seq.index s 0)
 {
-    arr.(0sz) // indices have type FStar.SizeT
+    arr.(0sz) // indices have type FStar.SizeT 
 }
 
 
 
+
 [@@expect_failure]
+
 fn read_spec_fails (arr:array int) (s:erased (seq int))
   requires pts_to arr s ** pure (Seq.length s > 0)
   returns x:int
   ensures pts_to arr s ** pure (x == Seq.index s 0)
 {
-    arr.(0sz) // indices have type FStar.SizeT
+    arr.(0sz) // indices have type FStar.SizeT 
 }
+
+
 
 
 fn write (s:erased (seq int)) (arr:array int) (x:int) (i:SizeT.t { v i < length s })
@@ -34,6 +39,8 @@ fn write (s:erased (seq int)) (arr:array int) (x:int) (i:SizeT.t { v i < length 
     arr.(i) <- x
 }
 
+
+
 fn mk_even (r:ref int)
   requires exists* v. R.pts_to r v
   ensures exists* w. R.pts_to r w ** pure (w % 2 == 0)
@@ -42,7 +49,9 @@ fn mk_even (r:ref int)
     r := n + n
 }
 
+
 // Elim and intro exists may be done explicitly as well
+
 
 fn mk_even_explicit (r:R.ref int)
   requires exists* v. R.pts_to r v
@@ -54,10 +63,12 @@ fn mk_even_explicit (r:R.ref int)
     introduce exists* w. R.pts_to r w ** pure (w % 2 == 0) with (v + v)
 }
 
+
 module A = Pulse.Lib.Array
 module BoundedInts = Pulse.Lib.BoundedIntegers
 
-fn compare (#t:eqtype) #p1 #p2 (a1 a2:A.array t) (l:SZ.t)
+
+fn compare (#t:eqtype) #p1 #p2 (a1 a2:A.array t) (l:SZ.t) 
   requires (
     A.pts_to a1 #p1 's1 **
     A.pts_to a2 #p2 's2 **
@@ -82,19 +93,18 @@ fn compare (#t:eqtype) #p1 #p2 (a1 a2:A.array t) (l:SZ.t)
       false
     }
   )
-  invariant b.
-  exists* vi. (
+  invariant
+  exists* vi. ( 
     R.pts_to i vi **
     A.pts_to a1 #p1 's1 **
     A.pts_to a2 #p2 's2 **
     pure (
       vi <= l /\
-      (b == (vi < l && Seq.index 's1 (v vi) = Seq.index 's2 (v vi))) /\
       (forall (i:nat). i < v vi ==> Seq.index 's1 i == Seq.index 's2 i)
     )
   )
   {
-    let vi = !i;
+    let vi = !i; 
     i := vi + 1sz
   };
   let vi = !i;
@@ -102,7 +112,9 @@ fn compare (#t:eqtype) #p1 #p2 (a1 a2:A.array t) (l:SZ.t)
 }
 //compareimplend$
 
+
 module Vec = Pulse.Lib.Vec
+
 fn test_compare ()
   requires emp
   ensures emp
@@ -110,13 +122,14 @@ fn test_compare ()
     let mut a1 = [| 0; 2sz |];  // stack array, allocated using the repeat constructor
 
     let a2 = Vec.alloc 0 2sz;  // heap allocated array
-
+    
     Vec.to_array_pts_to a2;  // explicit coercions from vec to array and back
     compare a1 (Vec.vec_to_array a2) 2sz;
     Vec.to_vec_pts_to a2;
 
     Vec.free a2  // need to free a2, a1 is automatically reclaimed when the function returns
 }
+
 
 // Exercise:
 // Here's an F* specification of a function that sums up the elements of a sequence
@@ -130,6 +143,7 @@ let rec sum_spec (s:Seq.seq int) : Tot int (decreases Seq.length s) =
 
 // Write a Pulse implementation of this function on arrays, proven to be equivalent
 // to the sequence spec above
+
 fn sum #p (#s:erased _) (arr:array int) (len:SZ.t { v len == Seq.length s })
   requires pts_to arr #p s
   returns res:int
@@ -138,3 +152,4 @@ fn sum #p (#s:erased _) (arr:array int) (len:SZ.t { v len == Seq.length s })
   open BoundedInts;
   admit()
 }
+
