src/tutorial/exercises/PulseTutorialExercises.TruncatePoint.fst
@@ -1,8 +1,7 @@
 module PulseTutorialExercises.TruncatePoint
 #lang-pulse
-open Pulse
+open Pulse.Lib.Pervasives
 open Pulse.Lib.Box
-module Box = Pulse.Lib.Box
 noeq
 type point = {
     x:box int;
@@ -12,6 +11,7 @@ type point = {
 let is_point (p:point) (xy:int & int) =
   pts_to p.x (fst xy) **
   pts_to p.y (snd xy)
+
 
 ghost
 fn fold_is_point (x y:box int) (#a #b:int)
@@ -24,6 +24,8 @@ ensures (is_point {x; y} (a, b))
     rewrite each p as ({x;y});
 }
 
+
+
 fn new_point (x y : int)
 requires emp
 returns p:point
@@ -32,11 +34,13 @@ ensures is_point p (x, y)
    admit()
 }
 
+
 let truncate (p1 p2: (int & int)) =
     let min x y = if x < y then x else y in
     let (x1, y1) = p1 in
     let (x2, y2) = p2 in
     min x1 x2, min y1 y2
+    
 
 fn trunc (p1 p2:point)
 requires is_point p1 'v1 ** is_point p2 'v2
