src/tutorial/solutions/PulseTutorialSolutions.TruncatePoint.fst
@@ -1,6 +1,6 @@
 module PulseTutorialSolutions.TruncatePoint
 #lang-pulse
-open Pulse
+open Pulse.Lib.Pervasives
 open Pulse.Lib.Box
 module Box = Pulse.Lib.Box
 noeq
@@ -13,6 +13,7 @@ let is_point (p:point) (xy:int & int) =
   pts_to p.x (fst xy) **
   pts_to p.y (snd xy)
 
+
 ghost
 fn fold_is_point (x y:box int) (#a #b:int)
 requires pts_to x a ** pts_to y b
@@ -23,6 +24,8 @@ ensures (is_point {x; y} (a, b))
     fold (is_point p (a, b));
     rewrite each p as ({x;y});
 }
+
+
 
 fn new_point (x y : int)
 requires emp
@@ -35,11 +38,13 @@ ensures is_point p (x, y)
    ({ x = b_x; y = b_y });
 }
 
+
 let truncate (p1 p2: (int & int)) =
     let min x y = if x < y then x else y in
     let (x1, y1) = p1 in
     let (x2, y2) = p2 in
     min x1 x2, min y1 y2
+    
 
 fn trunc (p1 p2:point)
 requires is_point p1 'v1 ** is_point p2 'v2
